more above threshold experiments

theories/diffpriv/examples/sparse_vector_technique.v
@@ -25,6 +25,7 @@ Section svt.
              ∗ { AUTH ∗ { ⊤ } qᵢ db { v . v < T } } f db qi { false ∗ AUTH }
 [or this:]
              { AUTH } f db qi { b : bool . if b = false then AUTH }
+             ∀ R , { AUTH } f db qi ~ f db' qi { b b' : bool . b = R -> b' R ∗ if b = false then AUTH }
      }  *)
   Definition above_threshold : val :=
     λ:"num" "den" "T",
@@ -68,11 +69,10 @@ Section svt.
                (∀ q, wp_sensitive (Val q) 1 dDB dZ -∗
                      AUTH -∗
                      ⤇ fill K (f' q) -∗
-                     ∀ R : bool,
                      WP (Val f) (Val q)
                        {{ v, ∃ v', ⤇ fill K (Val v') ∗
-                                   ⌜ v = SOMEV #R → v' = SOMEV #R ⌝ ∗
-                                   (⌜R = false⌝ -∗ AUTH)
+                                   ⌜ v = v' ⌝ ∗
+                                   (⌜ v = SOMEV #false⌝ -∗ AUTH)
                        }}
 
                )
@@ -82,13 +82,298 @@ Section svt.
     tp_bind (Laplace _ _ _). wp_bind (Laplace _ _ _).
     set (ε := (IZR num / IZR den)). replace ε with (ε / 2 + ε / 2) by real_solver.
     fold ε in εpos.
+    assert (IZR den ≠ 0) by admit.
+    assert (0 < IZR num / IZR (2 * den)) by admit.
+    assert (0 < IZR num / IZR (4 * den)) by admit.
     iDestruct (ec_split with "ε") as "[ε ε']". 1,2: real_solver.
     iApply (wp_couple_laplace _ _ 1%Z 1%Z with "[$rhs ε']") => //.
     1: apply Zabs_ind ; lia.
-    1: admit.
     { iApply ec_eq. 2: iFrame. subst ε. replace (IZR (2 * den)) with (2 * IZR den).
       2: qify_r ; zify_q ; lia.
-      field. admit. }
+      field. done. }
+    iIntros (T') "!> rhs" => /=...
+    tp_alloc as reset_r "reset_r". wp_alloc reset_l as "reset_l"...
+    iModIntro. iExists _. iFrame.
+    set (AUTH := (↯ (ε / 2) ∗ reset_r ↦ₛ #false ∗ reset_l ↦ #false)%I).
+    iExists AUTH. iFrame.
+    iIntros "%q q_sens (ε & reset_r & reset_l) rhs"... tp_load. wp_load...
+
+    tp_bind (q _). wp_bind (q _). rewrite /wp_sensitive.
+    iSpecialize ("q_sens" $! _ _ db db'). iSpecialize ("q_sens" with "rhs").
+    Unshelve. 2: lra.
+    (* iPoseProof (wp_frame_l with "[reset_r $q_sens]") as "q_sens". 1: iAssumption.
+       iPoseProof (wp_frame_l with "[reset_l $q_sens]") as "q_sens". 1: iAssumption.
+       iPoseProof (wp_frame_l with "[ε $q_sens]") as "q_sens". 1: iAssumption. *)
+    iApply (wp_strong_mono'' with "q_sens [-]").
+    iIntros (?) "(%vq_l & %vq_r & -> & rhs & %adj')" => /=...
+    assert (-1 <= vq_l - vq_r <= 1)%Z as [].
+    {
+      rewrite Rmult_1_l in adj'.
+      assert (dZ vq_l vq_r <= 1) as h by (etrans ; eauto).
+      revert h.
+      rewrite /dZ/distance Rabs_Zabs.
+      apply Zabs_ind ; intros ? h; split.
+      all: pose proof (le_IZR _ _ h) ; lia.
+    }
+
+    (* We want to case on whether the result is the one that will get released (pweq?) *)
+    (* destruct R eqn:HR. *)
+    (* NB: no point in casing on T' ≤ vq_l: that doesn't mean (Lap vq_l ε') will be above T'. *)
+
+    (* Case 1, where the result is above the threshold. We can get a (v_l v_r . v_l+1 = v_r) coupling
+     between Lap vq_l and Lap vq_r for ↯(2*ε') by adjacency of vq_l and vq_r. Hence, we get v_l and
+     v_r adjacent. Then, since v_l is above T', v_r = v_l+1 is above T'+1 (by adjacency of v_l and
+     v_r). *)
+    assert (∀ v_l v_r,
+               T' ≤ v_l →
+               v_l + 1 = v_r →
+               T'+1 ≤ v_r)%Z
+      as case1 by intuition lia.
+
+    (* Case 2, where the result is below the threshold. We can get an isometry-coupling for free.
+     Then, by adjacency of vq_l and vq_r, if the left is below, then the right is below too. *)
+    assert (∀ v_l v_r,
+               (¬ T' ≤ v_l) →
+               v_l + (vq_r - vq_l) = v_r →
+               (¬ T'+1 ≤ v_r))%Z
+      as case2 by intuition lia.
+
+    set
+      (goal := ↯ (ε / 2) ∗
+               reset_l ↦ #false ∗
+               reset_r ↦ₛ #false ∗
+               ⤇ fill K
+                 (let: "vi" := Laplace #num #(4 * den) #vq_r in
+                  if: #(T' + 1) ≤ "vi" then #reset_r <- #true;; InjR #true
+                  else InjR #false)%E
+               ⊢
+                 WP let: "vi" := Laplace #num #(4 * den) #vq_l in
+                    if: #T' ≤ "vi" then #reset_l <- #true;; InjR #true else InjR #false
+                    {{ v, ∃ v' : val, ⤇ fill K v' ∗ ⌜v = v'⌝ ∗ (⌜v = InjRV #false⌝ -∗ AUTH) }}).
+    (* sanity check: is this the current goal? *)
+    cut goal.
+    { intros h. iApply h. iFrame. }
+
+    (* Here's how to prove the above-T case alone, admitting the other case. *)
+    assert goal as _.
+    {
+      subst goal.
+      iIntros "(ε & reset_l & reset_r & rhs)".
+      tp_bind (Laplace _ _ _). wp_bind (Laplace _ _ _).
+
+      (* case 1 *)
+      (* A direct proof of this case with the appropriate coupling is commented out here. *)
+      iApply (wp_couple_laplace vq_l vq_r 1%Z 2%Z with "[$rhs $ε]") => //.
+      1: apply Zabs_ind ; lia.
+      { subst ε. replace (IZR (4 * den)) with (4 * IZR den). 2: qify_r ; zify_q ; lia. field. done. }
+      iIntros "!> %v_l rhs" => /=...
+      destruct_decide (@bool_decide_reflect (T' ≤ v_l)%Z _) as res_l.
+      - eapply (case1) in res_l => //. rewrite (bool_decide_eq_true_2 _ res_l)...
+        tp_store ; wp_store... iFrame. iModIntro ; iSplitR ; iIntros ; done.
+      -
+        (* the credits are gone, can't re-establish AUTH. *)
+        admit.
+    }
+
+    (* Here's how to prove the below-T case alone, admitting the other case. *)
+    assert goal as _.
+    {
+      subst goal.
+      iIntros "(ε & reset_l & reset_r & rhs)".
+      tp_bind (Laplace _ _ _). wp_bind (Laplace _ _ _).
+
+      (* case 2 *)
+      (* A direct proof of this case with the appropriate coupling is commented out here. *)
+      iMod ec_zero as "ε0".
+      iApply (wp_couple_laplace vq_l vq_r (vq_r - vq_l)%Z 0%Z with "[$rhs $ε0]") => //.
+      1: apply Zabs_ind ; lia.
+      1: lra.
+      iIntros "!> %v_l rhs" => /=...
+      destruct_decide (@bool_decide_reflect (T' ≤ v_l)%Z _) as res_l.
+      - wp_pures.
+        case_bool_decide as res_r => /=... all: try tp_store ; tp_pures ; wp_store...
+        + iFrame. iSplitR. 1: done. iModIntro. iIntros (?). exfalso. done.
+        + iFrame. iSplitR. 2: iModIntro ; iIntros ; exfalso ; done.
+          iPureIntro.
+          (* LHS was above T, but RHS was not, and we don't know enough about the relation between
+             LHS and RHS to rule out this case. *)
+          Fail lia.
+          admit.
+      - eapply case2 in res_l. 2: eauto.
+        rewrite (bool_decide_eq_false_2 _ res_l)...
+        iExists _. iFrame. subst ε. iSplitR. 1: done. iIntros "!> _". done.
+    }
+
+    (* This magic rule for the Laplacian allows us to consume the errors only if we need to.
+       Specifically, we get to split on whether we are above a threshold.
+       Φ is just there to get the points-to into the post condition and can probably be removed. *)
+    set (Magic := ∀ num den loc loc' k k' ε K
+                    (Hdist : (Z.abs (k + loc - loc') <= k')%Z) (Hε : ε = IZR num / IZR den) Φ,
+            ↯ (IZR k' * ε) -∗
+            ⤇ fill K (Laplace #num #den #loc') -∗
+            Φ -∗
+            ∀ T : Z,
+              WP Laplace #num #den #loc
+                {{ v_l, ∃ z_l : Z,
+                      ⌜ v_l = #z_l ⌝ ∗
+                      ∃ z_r : Z,
+                        ⤇ fill K (Val #(z_r)%Z) ∗
+                        Φ ∗
+                        if bool_decide (T ≤ z_l)%Z then
+                          ⌜ (z_r = z_l + k)%Z ⌝
+                        else ⌜ (z_r = z_l + (loc' - loc))%Z ⌝ ∗ ↯ (IZR k' * ε)
+        }}).
+
+    (* The Magic rule implies the goal. *)
+    assert (Magic → goal) as _.
+    { intros magic. subst goal Magic.
+      iIntros "(ε & reset_l & reset_r & rhs)".
+      tp_bind (Laplace _ _ _). wp_bind (Laplace _ _ _).
+
+      opose proof (magic num (4*den)%Z vq_l vq_r 1%Z 2%Z _ _ _ _ _) as magic' ; clear magic.
+      1: apply Zabs_ind ; lia.
+      1: reflexivity.
+
+      iPoseProof (magic' with "[ε] [$rhs] [-]") as "magic" ; clear magic'.
+      { iApply ec_eq. 2: iFrame. subst ε. replace (IZR (4 * den)) with (4 * IZR den).
+        2: qify_r ; zify_q ; lia. field. done. }
+      { iAssert (reset_l ↦ #false ∗ reset_r ↦ₛ #false)%I with "[$]" as "h". iExact "h". }
+      unshelve iApply (wp_mono with "magic").
+      1: exact T'.
+      iIntros "% (%z_l & -> & %z_r & rhs & [reset_l reset_r] & h) /="...
+
+      destruct_decide (@bool_decide_reflect (T' ≤ z_l)%Z _) as res_l.
+
+      - eapply case1 in res_l => //. iDestruct "h" as "->". rewrite (bool_decide_eq_true_2 _ res_l)...
+        tp_store ; wp_store... iFrame. iModIntro ; iSplitR ; iIntros ; done.
+      - eapply case2 in res_l. 2: eauto.
+        iDestruct "h" as "[-> ε]".
+        rewrite (bool_decide_eq_false_2 _ res_l)...
+        iExists _. iFrame. subst ε. iSplitR. 1: done. iIntros "!> _". iApply ec_eq. 2: iFrame.
+        replace (IZR (4 * den)) with (4 * IZR den). 2: qify_r ; zify_q ; lia. field. done.
+    }
+
+
+    (* An attempt at a point-wise version of Laplace coupling. *)
+    set (wp_couple_laplace_pw := ∀ (loc loc' k k' : Z)
+                                   (Hdist : (Z.abs (k + loc - loc') <= k')%Z)
+                                   (num den : Z) (ε ε' : R) K E,
+            IZR num / IZR den = ε →
+            0 < IZR num / IZR den →
+            ε' = (IZR k' * ε) →
+            ∀ RES : Z,
+              {{{ ⤇ fill K (Laplace #num #den #loc') ∗ ↯ ε' }}}
+                Laplace #num #den #loc @ E
+                {{{ (z_l : Z), RET #z_l; ∃ z_r : Z, ⤇ fill K #(z_r) ∗ ⌜z_l = RES → (z_r = RES+k)%Z⌝ }}}).
+
+    (* General point-wise rule.  *)
+    set (Pweq := ∀ (e e' : expr) K,
+            (∀ x : bool, ⤇ fill K e' -∗ WP e {{ v, ∃ v', ⤇ fill K (of_val v') ∗ ⌜v = NONEV → v' = NONEV⌝ ∗ ⌜v = SOMEV #x -> v' = SOMEV #x⌝}})
+            -∗
+            (⤇ fill K e' -∗ WP e {{ v, ⤇ fill K (of_val v) }})).
+
+    (* This is pretty rough, and relies on further admits. *)
+    assert (Pweq → goal) as _.
+
+    { intros pweq. clear Magic. subst goal Pweq.
+      iIntros "(ε & reset_l & reset_r & rhs)".
+
+      (* Prove the point-wise spec for Above Threshold instead. *)
+      cut (
+          ∀ RES : Z,
+            ↯ (ε / 2) ∗
+            reset_l ↦ #false ∗
+            reset_r ↦ₛ #false ∗
+            ⤇ fill K
+              (let: "vi" := Laplace #num #(4 * den) #vq_r in
+               if: #(T' + 1) ≤ "vi" then #reset_r <- #true;; InjR #true
+               else InjR #false)%E
+            ⊢
+              WP let: "vi" := Laplace #num #(4 * den) #vq_l in
+                if: #T' ≤ "vi" then #reset_l <- #true;; InjR #true else InjR #false
+                {{ v, ∃ v' : val, ⤇ fill K v' ∗ ⌜v = SOMEV #RES → v' = SOMEV #RES⌝ ∗ (⌜v = SOMEV #false⌝ -∗ AUTH) }}).
+
+      { intros h.
+        (* actually, not even pweq is strong enough as stated *)
+        Fail iApply pweq. Fail iApply h. give_up. }
+
+      intros z_l.
+      iIntros "(ε & reset_l & reset_r & rhs)".
+
+      tp_bind (Laplace _ _ _). wp_bind (Laplace _ _ _).
+
+      destruct_decide (@bool_decide_reflect (T' ≤ z_l)%Z _) as res_l.
+      (* case 1 *)
+      - assert wp_couple_laplace_pw as lap_pw by admit.
+        unshelve iApply (lap_pw vq_l vq_r 1%Z 2%Z with "[$rhs $ε]") => //.
+        1: exact z_l.
+        1: apply Zabs_ind ; lia.
+        { subst ε. replace (IZR (4 * den)) with (4 * IZR den). 2: qify_r ; zify_q ; lia. field. done. }
+        iIntros "!> %v_l (%v_r & rhs & %h_pw)" => /=...
+
+        opose proof (case1 _ _ res_l _) as res_r => //.
+        assert (v_l = z_l) as -> by admit.
+        rewrite (bool_decide_eq_true_2 _ res_l).
+        rewrite h_pw => //.
+        rewrite (bool_decide_eq_true_2 _ res_r)...
+        tp_store ; wp_store... iFrame. iModIntro ; iSplitR ; iIntros ; done.
+
+      (* case 2 *)
+      - iMod ec_zero as "ε0".
+        iApply (wp_couple_laplace vq_l vq_r (vq_r - vq_l)%Z 0%Z with "[$rhs $ε0]") => //.
+        1: apply Zabs_ind ; lia.
+        1: lra.
+        iIntros "!> %v_l rhs" => /=...
+        assert (v_l = z_l) as -> by admit.
+        destruct_decide (@bool_decide_reflect (T' ≤ z_l)%Z _) as res_l' ; [lia|].
+        eapply case2 in res_l'. 2: eauto.
+        rewrite (bool_decide_eq_false_2 _ res_l')...
+        iFrame. done.
+    }
+    Fail Qed.
+  Abort.
+
+  Lemma Rdiv_pos_pos x y a (div_pos: 0 < x/y) (den_pos : 0 < a) : 0 < x / (a*y).
+  Admitted.
+  Lemma Rdiv_nonneg_nonneg x y a (div_noneg: 0 <= x/y) (den_noneg : 0 <= a) : 0 <= x / (a*y).
+  Admitted.
+  Lemma Rdiv_pos_den_0 x y (div_pos : 0 < x/y) : ¬ y = 0.
+  Proof.
+    intro d0. rewrite d0 in div_pos. rewrite Rdiv_0_r in div_pos. lra.
+  Qed.
+
+  Lemma above_threshold_online_spec_pw (num den T : Z) (εpos : 0 < IZR num / IZR den) `(dDB : Distance DB) (db db' : DB) (adj : dDB db db' <= 1) K :
+    ↯ (IZR num / IZR den) -∗
+    ⤇ fill K ((Val above_threshold) #num #den #T (Val (inject db')))
+    -∗
+    WP (Val above_threshold) #num #den #T (Val (inject db))
+       {{ f, ∃ f' : val,
+             ⤇ fill K (Val f') ∗
+             ∃ AUTH : iProp Σ,
+               AUTH ∗
+               ( ∀ q, wp_sensitive (Val q) 1 dDB dZ -∗
+                      AUTH -∗
+                      ⤇ fill K (f' q) -∗
+                      ∀ R : bool,
+                        WP (Val f) (Val q)
+                          {{ v, ∃ v', ⤇ fill K (Val v') ∗
+                                      ⌜ v = SOMEV #R → v' = SOMEV #R ⌝ ∗
+                                      (⌜R = false ∧ v = v' ∧ v = SOMEV #R⌝ -∗ AUTH)
+               }} )
+       }}.
+  Proof with (tp_pures ; wp_pures).
+    iIntros "ε rhs". rewrite /above_threshold...
+    tp_bind (Laplace _ _ _). wp_bind (Laplace _ _ _).
+    set (ε := (IZR num / IZR den)). replace ε with (ε / 2 + ε / 2) by real_solver.
+    fold ε in εpos.
+    iDestruct (ec_split with "ε") as "[ε ε']". 1,2: real_solver.
+    iApply (wp_couple_laplace _ _ 1%Z 1%Z with "[$rhs ε']") => //.
+    1: apply Zabs_ind ; lia.
+    1: rewrite mult_IZR ; apply Rdiv_pos_pos. 1,2: real_solver.
+    { iApply ec_eq. 2: iFrame. subst ε. replace (IZR (2 * den)) with (2 * IZR den).
+      2: qify_r ; zify_q ; lia.
+      field. eapply Rdiv_pos_den_0 => //.
+    }
     iIntros (T') "!> rhs" => /=...
     tp_alloc as reset_r "reset_r". wp_alloc reset_l as "reset_l"...
     iModIntro. iExists _. iFrame.
@@ -112,50 +397,260 @@ Section svt.
       apply Zabs_ind ; intros ? h; split.
       all: pose proof (le_IZR _ _ h) ; lia.
     }
-    (* want to case on whether the result is the one that will get released (pweq) *)
+    (* case on whether the result is the one that will get released (pweq) *)
     destruct R eqn:HR.
-    (* could we have case'd on T' ≤ vq_l instead? *)
     - tp_bind (Laplace _ _ _). wp_bind (Laplace _ _ _).
-      (* set (ε := (IZR num / IZR den)). replace ε with (ε / 2 + ε / 2) by real_solver.
-         fold ε in εpos.
-         iDestruct (ec_split with "ε") as "[ε ε']". 1,2: real_solver. *)
       iApply (wp_couple_laplace vq_l vq_r 1%Z 2%Z with "[$rhs ε]") => //.
       1: apply Zabs_ind ; lia.
-      1: admit.
-      { subst ε. admit. }
+      1: rewrite mult_IZR ; apply Rdiv_pos_pos ; real_solver.
+      { subst ε. iApply ec_eq. 2: iFrame. rewrite mult_IZR. field. eapply Rdiv_pos_den_0 => //. }
       iIntros "%vi !> rhs" => /=...
       case_bool_decide (_ (T' + 1)%Z _) ; tp_pures ; try tp_store ; tp_pures. all: case_bool_decide...
       all: try tp_store ; try wp_store ; try tp_pures ; try wp_pures.
-      + iFrame. iModIntro.
-        iSplitR. 1: done. iIntros (h).
-        inversion h.
+      + iFrame. iModIntro. iSplitR. 1: done.
+        iIntros ((h_R & h_vv' & h_vR)). exfalso. inversion h_R.
       + exfalso. lia.
       + exfalso. lia.
-      + iFrame. iSplitR. 1: done. iModIntro. iIntros (h). done.
+      + iFrame. iSplitR. 1: done. iModIntro.
+        iIntros ((h_R & h_vv' & h_vR)). exfalso. inversion h_R.
     - tp_bind (Laplace _ _ _). wp_bind (Laplace _ _ _).
-      (* set (ε := (IZR num / IZR den)). replace ε with (ε / 2 + ε / 2) by real_solver.
-         fold ε in εpos.
-         iDestruct (ec_split with "ε") as "[ε ε']". 1,2: real_solver. *)
-      iApply (wp_couple_laplace vq_l vq_r (vq_r - vq_l)%Z 0%Z with "[$rhs]") => //.
+      iMod ec_zero as "ε0".
+      iApply (wp_couple_laplace vq_l vq_r (vq_r - vq_l)%Z 0%Z with "[$rhs ε0]") => //.
       1: apply Zabs_ind ; lia.
-      1: admit.
-      { rewrite Rmult_0_l. admit. }
+      1: rewrite mult_IZR ; apply Rdiv_pos_pos ; real_solver.
+      1: rewrite Rmult_0_l ; iFrame.
       iIntros "%vi !> rhs" => /=...
       case_bool_decide (_ (T' + 1)%Z _) ; tp_pures ; try tp_store ; tp_pures. all: case_bool_decide...
       all: try tp_store ; try wp_store ; try tp_pures ; try wp_pures.
-      + iFrame. iModIntro.
-        iSplitR. 1: done. iIntros (h).
-        inversion h.
-        (* lost connection between return values and R *)
-        give_up.
+      + iFrame. iModIntro. iSplitR. 1: done.
+        iIntros ((_h_R & h_vv' & h_vR)). exfalso. inversion h_vR.
       + exfalso. lia.
-      + iFrame. iSplitR. 1: done.
-        (* lost connection between return values and R *)
+      + iFrame. iModIntro. iSplitR. 1: done.
+        iIntros ((_h_R & h_vv' & h_vR)). exfalso. inversion h_vR.
+      + iFrame. done.
+  Qed.
+
+
+  Definition above_threshold_no_flag : val :=
+    λ:"num" "den" "T",
+      let: "T'" := Laplace "num" (#2*"den") "T" in
+      λ:"db" "qi",
+        let: "vi" := Laplace "num" (#4*"den") ("qi" "db") in
+        "T'" ≤ "vi".
+
+  Lemma above_threshold_online_no_flag_spec_pw (num den T : Z) (εpos : 0 < IZR num / IZR den) K :
+    ↯ (IZR num / IZR den) -∗
+    ⤇ fill K ((Val above_threshold_no_flag) #num #den #T)
+    -∗
+    WP (Val above_threshold_no_flag) #num #den #T
+       {{ f, ∃ f' : val,
+             ⤇ fill K (Val f') ∗
+             ∃ AUTH : iProp Σ,
+               AUTH ∗
+               ( ∀ `(dDB : Distance DB) (db db' : DB) (adj : dDB db db' <= 1)
+                   q, wp_sensitive (Val q) 1 dDB dZ -∗
+                      AUTH -∗
+                      ⤇ fill K (f' (Val (inject db')) q) -∗
+                      ∀ R : bool,
+                        WP (Val f) (Val (inject db)) (Val q)
+                          {{ v, ∃ v', ⤇ fill K (Val v') ∗
+                                      ⌜ v = #R → v' = #R ⌝ ∗
+                                      (⌜R = false⌝ -∗ AUTH)
+               }}
+               )
+       }}.
+  Proof with (tp_pures ; wp_pures).
+    iIntros "ε rhs". rewrite /above_threshold_no_flag...
+    tp_bind (Laplace _ _ _). wp_bind (Laplace _ _ _).
+    set (ε := (IZR num / IZR den)). replace ε with (ε / 2 + ε / 2) by real_solver.
+    fold ε in εpos.
+    iDestruct (ec_split with "ε") as "[ε ε']". 1,2: real_solver.
+    iApply (wp_couple_laplace _ _ 1%Z 1%Z with "[$rhs ε']") => //.
+    1: apply Zabs_ind ; lia.
+    1: rewrite mult_IZR ; apply Rdiv_pos_pos. 1,2: real_solver.
+    { iApply ec_eq. 2: iFrame. subst ε. replace (IZR (2 * den)) with (2 * IZR den).
+      2: qify_r ; zify_q ; lia.
+      field. eapply Rdiv_pos_den_0 => //. }
+    iIntros (T') "!> rhs" => /=...
+    iModIntro. iExists _. iFrame "rhs".
+    iExists (↯ (ε / 2))%I. iFrame "ε".
+    iIntros (?????) "%q q_sens ε rhs %R"...
+
+    tp_bind (q _) ; wp_bind (q _). rewrite /wp_sensitive.
+    iSpecialize ("q_sens" $! _ _ db db'). iSpecialize ("q_sens" with "rhs").
+    Unshelve. 2: lra.
+
+    iApply (wp_strong_mono'' with "q_sens [ε]") => //.
+    iIntros (?) "(%vq_l & %vq_r & -> & rhs & %adj')" => /=...
+    assert (-1 <= vq_l - vq_r <= 1)%Z as [].
+    {
+      rewrite Rmult_1_l in adj'.
+      assert (dZ vq_l vq_r <= 1) as h by (etrans ; eauto).
+      revert h. rewrite /dZ/distance Rabs_Zabs.
+      apply Zabs_ind ; intros ? h; split.
+      all: pose proof (le_IZR _ _ h) ; lia.
+    }
+    tp_bind (Laplace _ _ _). wp_bind (Laplace _ _ _).
+    (* case on whether the result is the one that will get released (pweq) *)
+    destruct R eqn:HR.
+    - iApply (wp_couple_laplace vq_l vq_r 1%Z 2%Z with "[$rhs ε]") => //.
+      1: apply Zabs_ind ; lia.
+      1: rewrite mult_IZR ; apply Rdiv_pos_pos ; real_solver.
+      { subst ε. iApply ec_eq. 2: iFrame. rewrite mult_IZR. field. eapply Rdiv_pos_den_0 => //. }
+      iIntros "%z_l !> rhs" => /=. tp_pures.
+      case_bool_decide (_ (T' + 1)%Z _)...
+      all: destruct_decide (bool_decide_reflect (T' ≤ z_l)%Z) as res_l.
+      all: iFrame "rhs" ; iModIntro.
+      + iSplitR => //. iIntros (h_R). exfalso. inversion h_R.
+      + exfalso. lia.
+      + exfalso. lia.
+      + iSplitR => //. iIntros (h_R). exfalso. inversion h_R.
+    - iMod ec_zero as "ε0".
+      iApply (wp_couple_laplace vq_l vq_r (vq_r - vq_l)%Z 0%Z with "[$rhs ε0]") => //.
+      1: apply Zabs_ind ; lia.
+      1: rewrite mult_IZR ; apply Rdiv_pos_pos ; real_solver.
+      1: rewrite Rmult_0_l ; iFrame.
+      iIntros "%z_l !> rhs" => /=...
+      case_bool_decide (_ (T' + 1)%Z _).
+      all: destruct_decide (bool_decide_reflect (T' ≤ z_l)%Z) as res_l ; iModIntro ; iFrame "rhs".
+      all: iSplitR ; [|by iFrame "ε"].
+      + iIntros (Rf). inversion Rf.
+      + exfalso. lia.
+      + iIntros (Rf). inversion Rf.
+      + done.
+  Qed.
+
+
+  Definition WP_PWEQ : iProp Σ :=
+    ∀ (e e' : expr) K,
+      (∀ RES : val, ⤇ fill K e' -∗
+                    WP e {{ v, ∃ v', ⤇ fill K (of_val v') ∗ ⌜v = RES -> v' = RES⌝}})
+      -∗
+      (⤇ fill K e' -∗ WP e {{ v, ⤇ fill K (of_val v) }}).
+
+  Lemma pweq_frame_nodep e e' K : WP_PWEQ -∗ ∀ (AUTH : iProp Σ),
+      (∀ RES : val,
+          ⤇ fill K e' -∗
+          WP e {{ v, ∃ v', ⤇ fill K (of_val v') ∗ ⌜v = RES -> v' = RES⌝ ∗ AUTH }}) ∗
+      ⤇ fill K e' -∗
+        WP e
+          {{ v, ⤇ fill K (Val v) ∗
+                AUTH
+               }}.
+  Proof.
+    iIntros "wp_pweq". iIntros (?) "[h rhs]".
+    rewrite /WP_PWEQ.
+    iSpecialize ("wp_pweq" $! e  e' K).
+    iSpecialize ("wp_pweq" with "[h]").
+    { iIntros (?) "rhs". iSpecialize ("h" $! RES). iSpecialize ("h" with "rhs").
+      iApply wp_mono. 2: iAssumption. iIntros "% (% & ? & ? & ?)". iFrame.
+    }
+    iSpecialize ("wp_pweq" with "rhs"). iApply (wp_mono with "wp_pweq").
+    iIntros. iFrame.
+    give_up.
+  Abort.
+
+  Definition magic_post :=
+    forall e Φ Ψ Ξ R,
+    (R -∗ WP e {{ v , Φ v ∗ Ξ v }}) ∗
+    ((R -∗ WP e {{ v , Φ v }}) -∗ R -∗ WP e {{ v , Ψ v}}) ⊢ R -∗ WP e {{ v , Ψ v ∗ Ξ v }}.
+
+
+  Lemma pweq_frame e e' K : WP_PWEQ -∗ ∀ (AUTH : val -> iProp Σ),
+      (∀ RES : val,
+          ⤇ fill K e' -∗
+          WP e {{ v, ∃ v', ⤇ fill K (of_val v') ∗ ⌜v = RES -> v' = RES⌝ ∗ AUTH RES }}) ∗
+      ⤇ fill K e' -∗
+        WP e
+          {{ v, ⤇ fill K (Val v) ∗
+                AUTH v
+               }}.
+  Proof.
+    iIntros "wp_pweq". iIntros (?) "h".
+    rewrite /WP_PWEQ.
+    iSpecialize ("wp_pweq" $! e  e' K).
+  Abort.
+
+
+  Lemma above_threshold_online_no_flag_spec_pw_no_AUTH (num den T : Z) (εpos : 0 < IZR num / IZR den) K :
+    ↯ (IZR num / (2 * IZR den)) -∗
+    ⤇ fill K ((Val above_threshold_no_flag) #num #den #T)
+    -∗
+    WP (Val above_threshold_no_flag) #num #den #T
+       {{ f, ∃ f' : val,
+             ⤇ fill K (Val f') ∗
+               ( ∀ `(dDB : Distance DB) (db db' : DB) (adj : dDB db db' <= 1)
+                   q, wp_sensitive (Val q) 1 dDB dZ -∗
+                      ⤇ fill K (f' (Val (inject db')) q) -∗
+                      ∀ R : bool, (if R then ↯ (IZR num / (2 * IZR den)) else emp) -∗
+                        WP (Val f) (Val (inject db)) (Val q)
+                          {{ v, ∃ v', ⤇ fill K (Val v') ∗
+                                      ⌜ v = v' ⌝
+               }} )
+       }}.
+  Proof with (tp_pures ; wp_pures).
+    iIntros "ε rhs". rewrite /above_threshold_no_flag...
+    tp_bind (Laplace _ _ _). wp_bind (Laplace _ _ _).
+    set (ε := (IZR num / 2 * IZR den)).
+    fold ε in εpos.
+    (* iDestruct (ec_split with "ε") as "[ε ε']". 1,2: real_solver. *)
+    iApply (wp_couple_laplace _ _ 1%Z 1%Z with "[$rhs ε]") => //.
+    1: apply Zabs_ind ; lia.
+    1: rewrite mult_IZR ; apply Rdiv_pos_pos. 1,2: real_solver.
+    { iApply ec_eq. 2: iFrame. subst ε. replace (IZR (2 * den)) with (2 * IZR den).
+      2: qify_r ; zify_q ; lia.
+      field. eapply Rdiv_pos_den_0 => //. }
+    iIntros (T') "!> rhs" => /=...
+    iModIntro. iExists _. iFrame "rhs".
+    (* iExists (↯ (ε / 2))%I. iFrame "ε". *)
+    iIntros (?????) "%q q_sens rhs %R ε" => /=...
+
+    tp_bind (q _) ; wp_bind (q _). rewrite /wp_sensitive.
+    iSpecialize ("q_sens" $! _ _ db db'). iSpecialize ("q_sens" with "rhs").
+    Unshelve. 2: lra.
+
+    iApply (wp_strong_mono'' with "q_sens [ε]") => //.
+    iIntros (?) "(%vq_l & %vq_r & -> & rhs & %adj')" => /=...
+    assert (-1 <= vq_l - vq_r <= 1)%Z as [].
+    {
+      rewrite Rmult_1_l in adj'.
+      assert (dZ vq_l vq_r <= 1) as h by (etrans ; eauto).
+      revert h. rewrite /dZ/distance Rabs_Zabs.
+      apply Zabs_ind ; intros ? h; split.
+      all: pose proof (le_IZR _ _ h) ; lia.
+    }
+    tp_bind (Laplace _ _ _). wp_bind (Laplace _ _ _).
+    (* case on whether the result is the one that will get released (pweq) *)
+    destruct R eqn:HR.
+    - iApply (wp_couple_laplace vq_l vq_r 1%Z 2%Z with "[$rhs ε]") => //.
+      1: apply Zabs_ind ; lia.
+      1: rewrite mult_IZR ; apply Rdiv_pos_pos ; real_solver.
+      { subst ε. iApply ec_eq. 2: iFrame. rewrite mult_IZR. field. eapply Rdiv_pos_den_0 => //. }
+      iIntros "%z_l !> rhs" => /=. tp_pures.
+      case_bool_decide (_ (T' + 1)%Z _)...
+      all: destruct_decide (bool_decide_reflect (T' ≤ z_l)%Z) as res_l.
+      all: iFrame "rhs" ; iModIntro.
+      + done.
+      + exfalso. lia.
+      + exfalso. lia.
+      + done.
+    - iMod ec_zero as "ε0".
+      iApply (wp_couple_laplace vq_l vq_r (vq_r - vq_l)%Z 0%Z with "[$rhs ε0]") => //.
+      1: apply Zabs_ind ; lia.
+      1: rewrite mult_IZR ; apply Rdiv_pos_pos ; real_solver.
+      1: rewrite Rmult_0_l ; iFrame.
+      iIntros "%z_l !> rhs" => /=...
+      case_bool_decide (_ (T' + 1)%Z _).
+      all: destruct_decide (bool_decide_reflect (T' ≤ z_l)%Z) as res_l ; iModIntro ; iFrame "rhs".
+      + done.
+      + exfalso. lia.
+      +
+        (* can't even seem to prove this *)
         give_up.
-      + iFrame. iSplitR. 1: done. done.
-
-
+      + done.
   Admitted.
+
+
 
   (* SVT calibrates the noise by simply dividing up the initial budget ε =
   num/den over the number of queries c exceeding the threshold T and running
